Generalize field assumptions in curve25519 proofs so far
This changes only the formal specification and its proof, with the
code itself being unchanged. The previous version of the spec, given
the input X, was degenerate unless there was a corresponding Y in the
prime field F(2^255-19) with the affine point (X,Y) on the curve. But
the curve25519 X-coordinate functions like x25519 are explicitly
intended to work even on X inputs where the only suitable Y lives in
an extension field, and the new specification is general over all
fields of characteristic 2^255-19. This includes in particular the
quadratic extension F(2^255-19)[sqrt(2)], which has square roots for
all elements of the prime field and is used in Bernstein's original

  https://cr.yp.to/ecdh/curve25519-20060209.pdf

x86/proofs/curve25519_pxscalarmul.ml
@@ -20,8 +20,7 @@
 needs "x86/proofs/base.ml";;
 needs "common/ecencoding.ml";;
 
-needs "EC/curve25519.ml";;
-needs "EC/formulary_xzprojective.ml";;
+needs "EC/x25519.ml";;
 
 prioritize_int();;
 prioritize_real();;
@@ -1811,24 +1810,19 @@ let CURVE25519_PXSCALARMUL_EXEC =
 
 let p_25519 = define `p_25519 = 57896044618658097711785492504343953926634992332820282019728792003956564819949`;;
 
-let curve25519 = define
- `curve25519 = (integer_mod_ring p_25519,&A_25519:int,&1:int)`;;
+let curve25519x = define
+ `curve25519x (f:A ring) = (f,ring_of_num f A_25519,ring_of_num f 1)`;;
 
-let curve25519_encode = new_definition
-  `curve25519_encode = modular_encode(256,p_25519)`;;
+let curve25519x_canonically_represents = new_definition
+ `curve25519x_canonically_represents (f:A ring) P (X,Z) <=>
+        X < p_25519 /\ Z < p_25519 /\
+        montgomery_xz f P (ring_of_num f X,ring_of_num f Z)`;;
 
-let curve25519_decode = new_definition
-  `curve25519_decode = modular_decode(256,p_25519)`;;
-
-let curve25519_represents = new_definition
- `curve25519_represents P (X,Z) <=>
-        montgomery_xz (integer_mod_ring p_25519) P (&X,&Z)`;;
-
-let CURVE25519_REPRESENTS_BOUND = prove
- (`!P X Z. curve25519_represents P (X,Z) ==> X < p_25519 /\ Z < p_25519`,
-  REWRITE_TAC[FORALL_OPTION_THM; FORALL_PAIR_THM; curve25519_represents] THEN
-  REWRITE_TAC[montgomery_xz; IN_INTEGER_MOD_RING_CARRIER] THEN
-  REWRITE_TAC[INT_OF_NUM_CLAUSES; p_25519] THEN ARITH_TAC);;
+let CURVE25519X_CANONICALLY_REPRESENTS_BOUND = prove
+ (`!(f:A ring) P X Z.
+        curve25519x_canonically_represents (f:A ring) P (X,Z)
+        ==> X < p_25519 /\ Z < p_25519`,
+  SIMP_TAC[curve25519x_canonically_represents]);;
 
 (* ------------------------------------------------------------------------- *)
 (* Common lemmas and tactics for the component proofs.                       *)
@@ -3117,57 +3111,58 @@ let lemma = prove
   REWRITE_TAC[INT_OF_NUM_LT; p_25519] THEN CONV_TAC NUM_REDUCE_CONV);;
 
 let lemma_double = prove
- (`P IN group_carrier curve25519_group /\
-   montgomery_xz (integer_mod_ring p_25519)
-     (group_pow curve25519_group P n) (&x,&y)
-   ==> montgomery_xz (integer_mod_ring p_25519)
-        (group_pow curve25519_group P (2 * n))
-           (montgomery_xzdouble curve25519 (&x,&y))`,
-  REWRITE_TAC[curve25519; curve25519_group] THEN REPEAT STRIP_TAC THEN
+ (`P IN group_carrier (curve25519x_group(f:A ring)) /\
+   montgomery_xz f (group_pow (curve25519x_group f) P n) (x,y)
+   ==> field f /\ ring_char f = p_25519
+       ==> montgomery_xz f
+            (group_pow (curve25519x_group f) P (2 * n))
+               (montgomery_xzdouble (curve25519x f) (x,y))`,
+  REWRITE_TAC[curve25519x; curve25519x_group] THEN REPEAT STRIP_TAC THEN
   MATCH_MP_TAC MONTGOMERY_XZDOUBLE_GROUP THEN ASM_REWRITE_TAC[] THEN
-  REWRITE_TAC[GSYM curve25519; MONTGOMERY_NONSINGULAR_CURVE25519] THEN
-  REWRITE_TAC[A_25519; p_25519; IN_INTEGER_MOD_RING_CARRIER;
-              FIELD_INTEGER_MOD_RING; INTEGER_MOD_RING_CHAR] THEN
-  CONV_TAC(DEPTH_CONV(INTEGER_MOD_RING_RED_CONV ORELSEC INT_RED_CONV)) THEN
-  REWRITE_TAC[ARITH_EQ] THEN REWRITE_TAC[GSYM p_25519; PRIME_P25519]);;
+  ASM_SIMP_TAC[GSYM curve25519x; MONTGOMERY_NONSINGULAR_CURVE25519X] THEN
+  REWRITE_TAC[A_25519; p_25519; RING_OF_NUM] THEN
+  CONV_TAC NUM_REDUCE_CONV);;
 
 let lemma_diffadd1 = prove
- (`~(&x:int = &0) /\
-   P IN group_carrier curve25519_group /\
-   montgomery_xz (integer_mod_ring p_25519) P (&x,&1) /\
-   montgomery_xz (integer_mod_ring p_25519)
-     (group_pow curve25519_group P (n + 1)) (&xn,&zn) /\
-   montgomery_xz (integer_mod_ring p_25519)
-     (group_pow curve25519_group P n) (&xm,&zm)
-   ==> montgomery_xz (integer_mod_ring p_25519)
-        (group_pow curve25519_group P (2 * n + 1))
-        (montgomery_xzdiffadd curve25519 (&x,&1) (&xn,&zn) (&xm,&zm))`,
-  REWRITE_TAC[curve25519; curve25519_group] THEN REPEAT STRIP_TAC THEN
+ (`field f /\ ring_char f = p_25519 /\
+   ~(x:A = ring_0 f) /\
+   P IN group_carrier (curve25519x_group f) /\
+   montgomery_xz f P (x,ring_of_num f 1) /\
+   montgomery_xz f
+     (group_pow (curve25519x_group f) P (n + 1)) (xn,zn) /\
+   montgomery_xz f
+     (group_pow (curve25519x_group f) P n) (xm,zm)
+   ==> montgomery_xz f
+            (group_pow (curve25519x_group f) P (2 * n + 1))
+            (montgomery_xzdiffadd (curve25519x f) (x,ring_of_num f 1)
+                  (xn,zn) (xm,zm))`,
+  REWRITE_TAC[curve25519x; curve25519x_group] THEN REPEAT STRIP_TAC THEN
   MATCH_MP_TAC MONTGOMERY_XZDIFFADD_GROUP THEN ASM_REWRITE_TAC[] THEN
-  REWRITE_TAC[GSYM curve25519; MONTGOMERY_NONSINGULAR_CURVE25519] THEN
-  REWRITE_TAC[A_25519; p_25519; IN_INTEGER_MOD_RING_CARRIER;
-              FIELD_INTEGER_MOD_RING; INTEGER_MOD_RING_CHAR] THEN
-  CONV_TAC(DEPTH_CONV(INTEGER_MOD_RING_RED_CONV ORELSEC INT_RED_CONV)) THEN
-  REWRITE_TAC[ARITH_EQ] THEN ASM_REWRITE_TAC[GSYM p_25519; PRIME_P25519]);;
+  ASM_SIMP_TAC[GSYM curve25519x; MONTGOMERY_NONSINGULAR_CURVE25519X] THEN
+  REWRITE_TAC[A_25519; p_25519; RING_OF_NUM] THEN
+  ASM_SIMP_TAC[RING_OF_NUM_1; FIELD_NONTRIVIAL] THEN
+  CONV_TAC NUM_REDUCE_CONV);;
 
 let lemma_diffadd2 = prove
- (`~(&x:int = &0) /\
-   P IN group_carrier curve25519_group /\
-   montgomery_xz (integer_mod_ring p_25519) P (&x,&1) /\
-   montgomery_xz (integer_mod_ring p_25519)
-     (group_pow curve25519_group P (n + 1)) (&xm,&zm) /\
-   montgomery_xz (integer_mod_ring p_25519)
-     (group_pow curve25519_group P n) (&xn,&zn)
-   ==> montgomery_xz (integer_mod_ring p_25519)
-        (group_pow curve25519_group P (2 * n + 1))
-        (montgomery_xzdiffadd curve25519 (&x,&1) (&xn,&zn) (&xm,&zm))`,
+ (`field f /\ ring_char f = p_25519 /\
+   ~(x:A = ring_0 f) /\
+   P IN group_carrier (curve25519x_group f) /\
+   montgomery_xz f P (x,ring_of_num f 1) /\
+   montgomery_xz f
+     (group_pow (curve25519x_group f) P (n + 1)) (xm,zm) /\
+   montgomery_xz f
+     (group_pow (curve25519x_group f) P n) (xn,zn)
+   ==> montgomery_xz f
+            (group_pow (curve25519x_group f) P (2 * n + 1))
+            (montgomery_xzdiffadd (curve25519x f) (x,ring_of_num f 1)
+                  (xn,zn) (xm,zm))`,
   DISCH_TAC THEN
   FIRST_ASSUM(MP_TAC o MATCH_MP lemma_diffadd1) THEN
   MATCH_MP_TAC EQ_IMP THEN AP_TERM_TAC THEN
   POP_ASSUM STRIP_ASSUME_TAC THEN
   REPEAT(FIRST_X_ASSUM(MP_TAC o MATCH_MP MONTGOMERY_XZ_IN_CARRIER)) THEN
-  ASM_SIMP_TAC[montgomery_xzdiffadd; curve25519; RING_MUL_SYM; PAIR_EQ] THEN
-  SPEC_TAC(`integer_mod_ring p_25519`,`r:int ring`) THEN RING_TAC);;
+  ASM_SIMP_TAC[montgomery_xzdiffadd; curve25519x; RING_MUL_SYM; PAIR_EQ] THEN
+  RING_TAC);;
 
 let CURVE25519_PXSCALARMUL_CORRECT = time prove
  (`!res point X scalar n pc stackpointer.
@@ -3182,10 +3177,12 @@ let CURVE25519_PXSCALARMUL_CORRECT = time prove
               bignum_from_memory (point,4) s = X /\
               bignum_from_memory (scalar,4) s = n)
          (\s. read RIP s = word (pc + 0x1625) /\
-              !P. P IN group_carrier curve25519_group /\
-                  curve25519_represents P (X,1)
-                  ==> curve25519_represents
-                        (group_pow curve25519_group P n)
+              !(f:A ring) P.
+                  field f /\ ring_char f = p_25519 /\
+                  P IN group_carrier(curve25519x_group f) /\
+                  curve25519x_canonically_represents f P (X,1)
+                  ==> curve25519x_canonically_represents f
+                        (group_pow (curve25519x_group f) P n)
                         (bignum_pair_from_memory(res,4) s))
           (MAYCHANGE [RIP; RDI; RAX; RBX; RCX; RDX; RBP;
                       R8; R9; R10; R11; R12; R13; R14; R15] ,,
@@ -3211,8 +3208,10 @@ let CURVE25519_PXSCALARMUL_CORRECT = time prove
       bignum_from_memory (scalar,4) s = nn /\
       read (memory :> bytes64(word_add stackpointer (word 352))) s =
       word(bitval(ODD(nn DIV 2 EXP i))) /\
-      !P. P IN group_carrier curve25519_group /\
-          curve25519_represents P (X,1)
+      !(f:A ring) P.
+        field f /\ ring_char f = p_25519 /\
+        P IN group_carrier(curve25519x_group f) /\
+        curve25519x_canonically_represents f P (X,1)
       ==>
       if X = 0 then
         bignum_from_memory(stackpointer,4) s <= 1 /\
@@ -3220,14 +3219,14 @@ let CURVE25519_PXSCALARMUL_CORRECT = time prove
         bignum_from_memory(word_add stackpointer (word 192),4) s = 0 /\
         bignum_from_memory(word_add stackpointer (word 256),4) s <= 1
       else
-      curve25519_represents
-       (group_pow curve25519_group P
+      curve25519x_canonically_represents f
+       (group_pow (curve25519x_group f) P
            (if ODD(nn DIV 2 EXP i)
             then nn DIV 2 EXP i + 1 else nn DIV 2 EXP i))
        (bignum_from_memory(word_add stackpointer (word 256),4) s,
         bignum_from_memory(word_add stackpointer (word 96),4) s) /\
-      curve25519_represents
-       (group_pow curve25519_group P
+      curve25519x_canonically_represents f
+       (group_pow (curve25519x_group f) P
           (if ODD(nn DIV 2 EXP i)
            then nn DIV 2 EXP i else nn DIV 2 EXP i + 1))
        (bignum_from_memory(word_add stackpointer (word 192),4) s,
@@ -3247,10 +3246,12 @@ let CURVE25519_PXSCALARMUL_CORRECT = time prove
     REWRITE_TAC[bignum_of_wordlist] THEN
     CONV_TAC(DEPTH_CONV WORD_NUM_RED_CONV) THEN
     ASM_SIMP_TAC[GROUP_POW_1] THEN REWRITE_TAC[group_pow] THEN
-    REPEAT STRIP_TAC THEN REWRITE_TAC[CURVE25519_GROUP] THEN
-    REWRITE_TAC[curve25519_represents; montgomery_xz] THEN
-    SIMP_TAC[p_25519; INTEGER_MOD_RING_CLAUSES; ARITH_LT] THEN
-    REWRITE_TAC[IN_ELIM_THM] THEN INT_ARITH_TAC;
+    SIMP_TAC[CURVE25519X_GROUP] THEN
+    REWRITE_TAC[curve25519x_canonically_represents; montgomery_xz] THEN
+    REWRITE_TAC[RING_OF_NUM] THEN
+    REWRITE_TAC[RING_OF_NUM_1; RING_OF_NUM_0; p_25519] THEN
+    SIMP_TAC[FIELD_NONTRIVIAL] THEN CONV_TAC NUM_REDUCE_CONV THEN
+    REWRITE_TAC[COND_ID];
 
     ALL_TAC; (*** The interesting part is done below ***)
 
@@ -3297,45 +3298,37 @@ let CURVE25519_PXSCALARMUL_CORRECT = time prove
     LOCAL_MUX_4_TAC 3 ["resx"; "xm"; "xn"] THEN
     LOCAL_MUX_4_TAC 0 ["resz"; "zm"; "zn"] THEN
     ENSURES_FINAL_STATE_TAC THEN ASM_REWRITE_TAC[] THEN
-    X_GEN_TAC `P:(int#int)option` THEN STRIP_TAC THEN
-    FIRST_X_ASSUM(MP_TAC o SPEC `P:(int#int)option`) THEN
+    MAP_EVERY X_GEN_TAC [`f:A ring`; `P:(A#A)option`] THEN STRIP_TAC THEN
+    FIRST_X_ASSUM(MP_TAC o SPECL [`f:A ring`; `P:(A#A)option`]) THEN
     ASM_REWRITE_TAC[WORD_RULE `word(8 * 4) = word 32`] THEN
     CONV_TAC(ONCE_DEPTH_CONV BIGNUM_LEXPAND_CONV) THEN
     ASM_REWRITE_TAC[] THEN
     ASM_CASES_TAC `X = 0` THEN
     ASM_REWRITE_TAC[BITVAL_CLAUSES; VAL_WORD_0; VAL_WORD_1] THENL
      [SUBGOAL_THEN
-       `group_pow curve25519_group P nn =
-        if EVEN nn then NONE else SOME(&0:int,&0)`
+       `group_pow (curve25519x_group (f:A ring)) P nn =
+        if EVEN nn then NONE else SOME(ring_0 f,ring_0 f)`
       SUBST1_TAC THENL
-       [UNDISCH_TAC `P IN group_carrier curve25519_group` THEN
-        FIRST_X_ASSUM(MP_TAC o GEN_REWRITE_RULE I [curve25519_represents]) THEN
-        SPEC_TAC(`P:(int#int)option`,`P:(int#int)option`) THEN
+       [UNDISCH_TAC `P IN group_carrier (curve25519x_group(f:A ring))` THEN
+        FIRST_X_ASSUM(MP_TAC o last o CONJUNCTS o GEN_REWRITE_RULE I
+         [curve25519x_canonically_represents]) THEN
+        SPEC_TAC(`P:(A#A)option`,`P:(A#A)option`) THEN
         ASM_REWRITE_TAC[montgomery_xz; FORALL_OPTION_THM; FORALL_PAIR_THM] THEN
-        REWRITE_TAC[p_25519; IN_INTEGER_MOD_RING_CARRIER] THEN
-        CONV_TAC(DEPTH_CONV
-         (INTEGER_MOD_RING_RED_CONV ORELSEC INT_RED_CONV)) THEN
-        REWRITE_TAC[CURVE25519_GROUP; IN] THEN
-        MAP_EVERY X_GEN_TAC [`x:int`; `z:int`] THEN
-        DISCH_THEN(SUBST1_TAC o SYM) THEN
-        MP_TAC MONTGOMERY_STRONGLY_NONSINGULAR_CURVE25519 THEN
-        REWRITE_TAC[curve25519] THEN
-        W(MP_TAC o PART_MATCH (lhand o rand) MONTGOMERY_STRONGLY_NONSINGULAR o
-          lhand o snd) THEN
-        REWRITE_TAC[A_25519; p_25519; IN_INTEGER_MOD_RING_CARRIER;
-                    FIELD_INTEGER_MOD_RING; INTEGER_MOD_RING_CHAR] THEN
-        CONV_TAC(DEPTH_CONV
-         (INTEGER_MOD_RING_RED_CONV ORELSEC INT_RED_CONV)) THEN
-        REWRITE_TAC[ARITH_EQ] THEN REWRITE_TAC[GSYM p_25519; PRIME_P25519] THEN
-        DISCH_THEN SUBST1_TAC THEN
-        DISCH_THEN(fun th -> DISCH_TAC THEN
-             MP_TAC(SPECL [`&0:int`; `z:int`] th) THEN ASM_REWRITE_TAC[]) THEN
-        DISCH_THEN SUBST1_TAC THEN SPEC_TAC(`nn:num`,`n:num`) THEN
-        POP_ASSUM_LIST(K ALL_TAC) THEN INDUCT_TAC THEN
+        ASM_SIMP_TAC[CURVE25519X_GROUP; RING_OF_NUM_0] THEN
+        REWRITE_TAC[SET_RULE `SOME p IN s <=> s(SOME p)`] THEN
+        SIMP_TAC[ring_div; RING_MUL_LZERO; RING_OF_NUM; RING_INV] THEN
+        ASM_SIMP_TAC[RING_0; RING_OF_NUM_1; FIELD_NONTRIVIAL] THEN
+        REWRITE_TAC[RIGHT_FORALL_IMP_THM; FORALL_UNWIND_THM1] THEN
+        X_GEN_TAC `y:A` THEN REWRITE_TAC[GSYM RING_OF_NUM_0] THEN
+        DISCH_TAC THEN
+        MP_TAC(ISPECL [`f:A ring`; `0:num`; `y:A`]
+         SPECIALLY_NONSINGULAR_CURVE25519X) THEN
+        ASM_REWRITE_TAC[RING_OF_NUM_0] THEN DISCH_THEN SUBST1_TAC THEN
+        SPEC_TAC(`nn:num`,`n:num`) THEN INDUCT_TAC THEN
         ASM_REWRITE_TAC[ARITH_EVEN; EVEN; COND_SWAP; group_pow] THEN
-        REWRITE_TAC[el 1 (CONJUNCTS CURVE25519_GROUP)] THEN
-        COND_CASES_TAC THEN ASM_REWRITE_TAC[] THEN
-        CONV_TAC(LAND_CONV ECGROUP_MUL_CONV) THEN REFL_TAC;
+        ASM_SIMP_TAC[CURVE25519X_GROUP] THEN
+        COND_CASES_TAC THEN
+        ASM_REWRITE_TAC[montgomery_add; curve25519x];
         ALL_TAC] THEN
       MAP_EVERY EXPAND_TAC ["zm"; "xn"] THEN
       REWRITE_TAC[ARITH_RULE `n <= 1 <=> n = 0 \/ n = 1`] THEN
@@ -3349,10 +3342,10 @@ let CURVE25519_PXSCALARMUL_CORRECT = time prove
       COND_CASES_TAC THEN ASM_REWRITE_TAC[] THEN
       STRIP_TAC THEN ASM_REWRITE_TAC[bignum_of_wordlist] THEN
       CONV_TAC(DEPTH_CONV WORD_NUM_RED_CONV) THEN
-      REWRITE_TAC[curve25519_represents; montgomery_xz] THEN
-      REWRITE_TAC[IN_INTEGER_MOD_RING_CARRIER; p_25519] THEN
-      CONV_TAC(DEPTH_CONV
-       (INTEGER_MOD_RING_RED_CONV ORELSEC INT_RED_CONV));
+      REWRITE_TAC[curve25519x_canonically_represents; montgomery_xz] THEN
+      ASM_SIMP_TAC[RING_OF_NUM_1; RING_OF_NUM_0; FIELD_NONTRIVIAL; ring_div;
+                   RING_0; RING_1; RING_MUL_LZERO; RING_INV; RING_1] THEN
+      REWRITE_TAC[p_25519] THEN CONV_TAC NUM_REDUCE_CONV;
       ASM_REWRITE_TAC[WORD_OR_0; VAL_WORD_BITVAL; BITVAL_EQ_0; COND_SWAP] THEN
       COND_CASES_TAC THEN ASM_REWRITE_TAC[] THEN SIMP_TAC[]]] THEN
 
@@ -3432,8 +3425,8 @@ let CURVE25519_PXSCALARMUL_CORRECT = time prove
 
   (*** Get started and handle the degenerate X = 0 case ***)
 
-  X_GEN_TAC `P:(int#int)option` THEN STRIP_TAC THEN
-  FIRST_X_ASSUM(MP_TAC o SPEC `P:(int#int)option`) THEN
+  MAP_EVERY X_GEN_TAC [`f:A ring`; `P:(A#A)option`] THEN STRIP_TAC THEN
+  FIRST_X_ASSUM(MP_TAC o SPECL [`f:A ring`; `P:(A#A)option`]) THEN
   ASM_REWRITE_TAC[] THEN COND_CASES_TAC THEN ASM_REWRITE_TAC[] THENL
    [FIRST_X_ASSUM SUBST_ALL_TAC THEN
     DISCH_THEN(REPEAT_TCL CONJUNCTS_THEN
@@ -3461,6 +3454,8 @@ let CURVE25519_PXSCALARMUL_CORRECT = time prove
     REWRITE_TAC[p_25519] THEN CONV_TAC INT_REDUCE_CONV;
     ALL_TAC] THEN
 
+  RULE_ASSUM_TAC(ONCE_REWRITE_RULE[TAUT
+   `(ODD n <=> b) <=> (b <=> ODD n)`]) THEN
   ABBREV_TAC `n = nn DIV 2 EXP (i + 1)` THEN
   ABBREV_TAC `b = ODD(nn DIV 2 EXP i)` THEN
   SUBGOAL_THEN `nn DIV 2 EXP i = 2 * n + bitval b` SUBST1_TAC THENL
@@ -3470,13 +3465,20 @@ let CURVE25519_PXSCALARMUL_CORRECT = time prove
 
   DISCH_TAC THEN
   SUBGOAL_THEN
-   `(&xm',&zm') = montgomery_xzdiffadd curve25519 (&X,&1) (&xn,&zn) (&xm,&zm) /\
-    (&xn',&zn') = montgomery_xzdouble curve25519
-                  (if b <=> ODD n then (&xn,&zn) else (&xm,&zm))`
+   `(ring_of_num f xm':A,ring_of_num f zm') =
+     montgomery_xzdiffadd (curve25519x f)
+         (ring_of_num f X,ring_of_num f 1)
+         (ring_of_num f xn,ring_of_num f zn)
+         (ring_of_num f xm,ring_of_num f zm) /\
+    (ring_of_num f xn',ring_of_num f zn') =
+     montgomery_xzdouble (curve25519x f)
+      (if b <=> ODD n then (ring_of_num f xn,ring_of_num f zn)
+       else (ring_of_num f xm,ring_of_num f zm))`
   MP_TAC THENL
-   [FIRST_X_ASSUM(CONJUNCTS_THEN
-     (STRIP_ASSUME_TAC o MATCH_MP CURVE25519_REPRESENTS_BOUND)) THEN
-    FIRST_X_ASSUM(STRIP_ASSUME_TAC o MATCH_MP CURVE25519_REPRESENTS_BOUND) THEN
+   [FIRST_X_ASSUM(CONJUNCTS_THEN (STRIP_ASSUME_TAC o
+      MATCH_MP CURVE25519X_CANONICALLY_REPRESENTS_BOUND)) THEN
+    FIRST_X_ASSUM(STRIP_ASSUME_TAC o
+      MATCH_MP CURVE25519X_CANONICALLY_REPRESENTS_BOUND) THEN
     REPEAT(FIRST_X_ASSUM(MP_TAC o check (is_imp o concl))) THEN
     REPEAT(ANTS_TAC THENL
      [ASM_REWRITE_TAC[] THEN SIMPLE_ARITH_TAC; STRIP_TAC]) THEN
@@ -3484,8 +3486,12 @@ let CURVE25519_PXSCALARMUL_CORRECT = time prove
     POP_ASSUM_LIST(MP_TAC o end_itlist CONJ o rev) THEN
     COND_CASES_TAC THEN
     ASM_REWRITE_TAC[montgomery_xzdiffadd; montgomery_xzdouble;
-                    curve25519; PAIR_EQ] THEN
-    STRIP_TAC THEN REWRITE_TAC[INTEGER_MOD_RING_CLAUSES; modular_encode] THEN
+                    curve25519x; PAIR_EQ] THEN
+    STRIP_TAC THEN
+    REWRITE_TAC[GSYM RING_OF_INT_OF_NUM; RING_OF_INT_CLAUSES] THEN
+    ASM_REWRITE_TAC[RING_OF_INT_EQ] THEN
+    REWRITE_TAC[GSYM INT_OF_NUM_REM; GSYM INT_REM_EQ;
+                GSYM INT_OF_NUM_CLAUSES] THEN
     CONV_TAC INT_REM_DOWN_CONV THEN
     REWRITE_TAC[PAIR_EQ; GSYM INT_OF_NUM_EQ; nintlemma] THEN
     REWRITE_TAC[GSYM INT_OF_NUM_REM; GSYM INT_OF_NUM_CLAUSES] THEN
@@ -3498,29 +3504,38 @@ let CURVE25519_PXSCALARMUL_CORRECT = time prove
     ASM_REWRITE_TAC[] THEN CONV_TAC INT_REM_DOWN_CONV THEN
     REPEAT CONJ_TAC THEN AP_THM_TAC THEN AP_TERM_TAC THEN
     REWRITE_TAC[A_25519] THEN INT_ARITH_TAC;
-    ASM_REWRITE_TAC[] THEN SIMP_TAC[curve25519_represents] THEN
-    DISCH_THEN(K ALL_TAC) THEN
-    FIRST_X_ASSUM(MP_TAC o GEN_REWRITE_RULE BINOP_CONV
-     [curve25519_represents]) THEN
-    FIRST_X_ASSUM(MP_TAC o GEN_REWRITE_RULE I [curve25519_represents]) THEN
-    UNDISCH_TAC `P IN group_carrier curve25519_group` THEN
-    UNDISCH_TAC `~(X = 0)` THEN POP_ASSUM_LIST(K ALL_TAC)] THEN
+    ASM_REWRITE_TAC[] THEN SIMP_TAC[curve25519x_canonically_represents] THEN
+    DISCH_THEN(K ALL_TAC) THEN REWRITE_TAC[MOD_LT_EQ; p_25519; ARITH_EQ] THEN
+    FIRST_X_ASSUM(CONJUNCTS_THEN(MP_TAC o last o CONJUNCTS o GEN_REWRITE_RULE I
+     [curve25519x_canonically_represents])) THEN
+    GEN_REWRITE_TAC I [GSYM IMP_CONJ_ALT] THEN
+    FIRST_X_ASSUM(MP_TAC o GEN_REWRITE_RULE I
+     [curve25519x_canonically_represents]) THEN
+    DISCH_THEN(CONJUNCTS_THEN2 ASSUME_TAC (MP_TAC o CONJUNCT2)) THEN
+    UNDISCH_TAC `P IN group_carrier(curve25519x_group(f:A ring))`] THEN
+
+  SUBGOAL_THEN `~(ring_of_num (f:A ring) X = ring_0 f)` MP_TAC THENL
+   [ASM_REWRITE_TAC[RING_OF_NUM_EQ_0] THEN
+    DISCH_THEN(MP_TAC o MATCH_MP DIVIDES_LE) THEN
+    ASM_REWRITE_TAC[NOT_LE];
+    MAP_EVERY UNDISCH_TAC
+     [`ring_char(f:A ring) = p_25519`; `field(f:A ring)`] THEN
+    POP_ASSUM_LIST(K ALL_TAC)] THEN
 
   REPEAT DISCH_TAC THEN CONJ_TAC THENL
    [DISJ_CASES_THEN SUBST_ALL_TAC (TAUT `(b <=> ODD n) \/ (b <=> ~ODD n)`) THEN
     REWRITE_TAC[TAUT `~(~p <=> p)`] THENL
      [FIRST_X_ASSUM(MP_TAC o CONJUNCT1);
       FIRST_X_ASSUM(MP_TAC o CONJUNCT2)] THEN
-    UNDISCH_TAC `P IN group_carrier curve25519_group` THEN
+    UNDISCH_TAC `P IN group_carrier(curve25519x_group(f:A ring))` THEN
     REWRITE_TAC[IMP_IMP] THEN DISCH_THEN(MP_TAC o MATCH_MP lemma_double) THEN
-    REWRITE_TAC[COND_SWAP] THEN COND_CASES_TAC THEN
+    ASM_REWRITE_TAC[COND_SWAP] THEN COND_CASES_TAC THEN
     REWRITE_TAC[ARITH_RULE `(2 * n + 1) + 1 = 2 * (n + 1)`];
 
     REPEAT(POP_ASSUM MP_TAC) THEN
     REWRITE_TAC[IMP_IMP; GSYM CONJ_ASSOC] THEN
-    COND_CASES_TAC THEN ASM_REWRITE_TAC[GSYM INT_OF_NUM_EQ] THEN
-    REWRITE_TAC[lemma_diffadd1] THEN
-    GEN_REWRITE_TAC (LAND_CONV o funpow 3 RAND_CONV) [CONJ_SYM] THEN
+    COND_CASES_TAC THEN REWRITE_TAC[lemma_diffadd1] THEN
+    GEN_REWRITE_TAC (LAND_CONV o funpow 5 RAND_CONV) [CONJ_SYM] THEN
     REWRITE_TAC[lemma_diffadd2]]);;
 
 let CURVE25519_PXSCALARMUL_SUBROUTINE_CORRECT = time prove
@@ -3539,10 +3554,12 @@ let CURVE25519_PXSCALARMUL_SUBROUTINE_CORRECT = time prove
               bignum_from_memory (scalar,4) s = n)
          (\s. read RIP s = returnaddress /\
               read RSP s = word_add stackpointer (word 8) /\
-              !P. P IN group_carrier curve25519_group /\
-                  curve25519_represents P (X,1)
-                  ==> curve25519_represents
-                        (group_pow curve25519_group P n)
+              !(f:A ring) P.
+                  field f /\ ring_char f = p_25519 /\
+                  P IN group_carrier(curve25519x_group f) /\
+                  curve25519x_canonically_represents f P (X,1)
+                  ==> curve25519x_canonically_represents f
+                        (group_pow (curve25519x_group f) P n)
                         (bignum_pair_from_memory(res,4) s))
           (MAYCHANGE [RIP; RSP; RDI; RAX; RCX; RDX; R8; R9; R10; R11] ,,
            MAYCHANGE SOME_FLAGS ,,
@@ -3576,10 +3593,12 @@ let WINDOWS_CURVE25519_PXSCALARMUL_SUBROUTINE_CORRECT = time prove
               bignum_from_memory (scalar,4) s = n)
          (\s. read RIP s = returnaddress /\
               read RSP s = word_add stackpointer (word 8) /\
-              !P. P IN group_carrier curve25519_group /\
-                  curve25519_represents P (X,1)
-                  ==> curve25519_represents
-                        (group_pow curve25519_group P n)
+              !(f:A ring) P.
+                  field f /\ ring_char f = p_25519 /\
+                  P IN group_carrier(curve25519x_group f) /\
+                  curve25519x_canonically_represents f P (X,1)
+                  ==> curve25519x_canonically_represents f
+                        (group_pow (curve25519x_group f) P n)
                         (bignum_pair_from_memory(res,4) s))
           (MAYCHANGE [RIP; RSP; RAX; RCX; RDX; R8; R9; R10; R11] ,,
            MAYCHANGE SOME_FLAGS ,,
